some elpi progress

tests/PrenexPoly.v
@@ -7,28 +7,29 @@ Elpi Db types.db lp:{{
 Elpi Command get_types.
 Elpi Accumulate Db types.db.
 Elpi Accumulate lp:{{
+  pred setly o:term.
+  setly X :- types X, coq.typecheck X Ty ok, Ty = {{ Set }}.
   main [] :- 
-    std.findall (types _) L, 
-    coq.say "The current set of types is" L.
+    std.findall (setly _) LS,
+    coq.say "The current set of setly types is" LS.
 }}.
 Elpi Typecheck.
-
-Elpi get_types.
 
 Elpi Command add_type.
 Elpi Accumulate Db types.db.
 Elpi Accumulate lp:{{
-  main [str Nme] :- 
-    coq.locate Nme GR,
+  main [trm Trm] :- 
     coq.elpi.accumulate _ "types.db" 
-      (clause _ _ (types (global GR))).
+      (clause _ _ (types Trm)).
 }}.
 Elpi Typecheck.
 
-Elpi get_types. (* prints [] *)
-Elpi add_type "nat".
-Elpi add_type "list".
-Elpi get_types. (* prints [types global indt «nat», types global indt «list»] *)
+Elpi add_type (nat).
+Elpi add_type (list).
+Elpi add_type (True).
+Elpi add_type (list nat).
+Elpi get_types.
+(* prints [types global indt «nat», types global indt «list»] *)
 
 Require Import Coq.Lists.List.
 Import ListNotations.
@@ -200,12 +201,118 @@ Definition bool_idx : list_idx tys_list := LIThere (LIHere).
 Definition add_func : funs _ [nat_idx; nat_idx] nat_idx := Nat.add.
 Require Import MirrorSolve.Reflection.Tactics.
 
+
 Notation sig := (sig_extensible tys_list).
 Notation mod := (mod_extensible tys_list).
 
 Definition sorts_eq_dec :  EquivDec.EqDec (sig_sorts sig) eq := eqdec_all.
 
+(* 
+  This is the reflection theorem for converting Coq Props (as quoted terms) to interpretations of FOL terms.
+  The brittle part has been sig and mod -- we've been using bespoke inductive types so far.
+  *)
 Check @denote_extract_specialized_rev sig mod sorts_eq_dec.
 
 Eval vm_compute in sorts_eq_dec bool_idx bool_idx.
 
+
+(* let's do the following goal: 
+   forall {A} (xs: list A), 
+    app' xs [] = xs 
+
+  (where app' is list append)
+*)
+
+Fixpoint app' {A: Type} (xs ys : list A) :=  
+  match xs with 
+  | [] => ys
+  | x :: xs => x :: app' xs ys
+  end.
+
+Elpi Tactic mirrorsolve.
+Elpi Accumulate lp:{{
+
+  pred setly i: term.
+  setly X :- coq.say "setly with" X, fail.
+  setly X :- coq.typecheck X Ty ok, Ty = {{ Set }}.
+  setly X :- coq.typecheck X Ty ok, Ty = {{ Type }}.
+
+  pred add_all i: list term i: std.set term o: std.set term.
+  add_all [] O O.
+  add_all [T|TS] S O :- 
+    add_all TS S O', 
+    std.set.add T O' O.
+
+  pred union_all i: list (std.set term) o: std.set term.
+  union_all [] O :- std.set.make _ O.
+  union_all [S|SS] O :- 
+    union_all SS O', 
+    add_all T O' O.
+
+  pred union i:std.set term i:std.set term o: std.set term.
+  union L R O :- 
+    std.set.elements L LS,
+    add_all LS R O.
+
+  pred gather_sorts_ls i: list term o: std.set term.
+  gather_sorts_ls [] O :- std.set.make _ O.
+  gather_sorts_ls [T|TS] O :- 
+    coq.say "recursing on term" T,
+    gather_sorts T O'',
+    gather_sorts_ls TS O',
+    union O'' O' O.
+
+  pred single i:term o: std.set term.
+  single X _ :- coq.say "singleton with" X, fail.
+  single X O :- 
+    std.set.make _ Empty,
+    std.set.add X Empty O. 
+  pred gather_sorts_term i: term o: std.set term.
+  gather_sorts_term T O :- setly T, coq.say T "is setly", single T O.
+  gather_sorts_term T O :- coq.say T "is not setly", std.set.make _ O.
+
+
+  pred gather_sorts i:term o:std.set term.
+  gather_sorts (app TS as G) GO :- 
+    gather_sorts_term G GO', 
+    gather_sorts_ls TS GO'',
+    union GO' GO'' GO.
+  gather_sorts G GO :- gather_sorts_term G GO.
+
+  pred setly_evar i: prop o:std.set term.
+  setly_evar X _ :- coq.say "setly_evar with" X, fail.
+  setly_evar (decl X _ _) O :- setly X, single X O.
+  setly_evar _ O :- std.set.make _ O.
+
+  pred setly_evars i: list prop o: std.set term.
+  setly_evars X _ :- coq.say "setly_evars with" X, fail.
+  setly_evars [] O :- std.set.make _ O.
+  setly_evars [X|XS] O :- 
+    setly_evar X O',
+    setly_evars XS O'',
+    union O' O'' O.
+
+  solve (goal Vs _ G' _ _ as G) GL :- 
+    % gather_sorts G' O,
+    % gather_sorts G' O, 
+    % std.set.elements O LS,
+    % gather_sorts G' O, 
+    setly_evars Vs O,
+    % std.set.cardinal O N,
+    std.set.elements O L,
+
+    coq.say "the evars are" Vs "and the setly vars are" L.
+}}.
+Elpi Typecheck.
+
+Ltac mirrorsolve' := admit.
+
+(* Elpi Trace.  *)
+Lemma app'_nil_r: 
+  forall {A} (xs: list A), app' xs [] = xs.
+Proof.
+  intros.
+  elpi mirrorsolve. (* for sorts, we expect A, list A *)
+  (* ideally the following proof: *)
+  induction xs; mirrorsolve'.
+Admitted.
